cedar-lean/Cedar/Thm/Partial/Evaluation.lean
@@ -1,0 +1,131 @@
+/-
+ Copyright Cedar Contributors
+
+ Licensed under the Apache License, Version 2.0 (the "License");
+ you may not use this file except in compliance with the License.
+ You may obtain a copy of the License at
+
+      https://www.apache.org/licenses/LICENSE-2.0
+
+ Unless required by applicable law or agreed to in writing, software
+ distributed under the License is distributed on an "AS IS" BASIS,
+ WITHOUT WARRANTIES OR CONDITIONS OF ANY KIND, either express or implied.
+ See the License for the specific language governing permissions and
+ limitations under the License.
+-/
+
+import Cedar.Partial.Evaluator
+import Cedar.Spec.Evaluator
+import Cedar.Thm.Partial.Evaluation.And
+import Cedar.Thm.Partial.Evaluation.Basic
+import Cedar.Thm.Partial.Evaluation.Binary
+import Cedar.Thm.Partial.Evaluation.Call
+import Cedar.Thm.Partial.Evaluation.GetAttr
+import Cedar.Thm.Partial.Evaluation.HasAttr
+import Cedar.Thm.Partial.Evaluation.Ite
+import Cedar.Thm.Partial.Evaluation.Or
+import Cedar.Thm.Partial.Evaluation.Record
+import Cedar.Thm.Partial.Evaluation.Set
+import Cedar.Thm.Partial.Evaluation.Unary
+import Cedar.Thm.Partial.Evaluation.Var
+import Cedar.Thm.Data.Control
+
+/-! This file contains theorems about Cedar's partial evaluator. -/
+
+namespace Cedar.Thm.Partial.Evaluation
+
+open Cedar.Data
+open Cedar.Partial (Unknown)
+open Cedar.Spec (Error Result)
+
+/--
+  Partial evaluation with concrete inputs gives the same output as
+  concrete evaluation with those inputs
+-/
+theorem on_concrete_eqv_concrete_eval (expr : Spec.Expr) (request : Spec.Request) (entities : Spec.Entities)
+  (wf : request.WellFormed) :
+  PartialEvalEquivConcreteEval expr request entities
+:= by
+  unfold PartialEvalEquivConcreteEval
+  cases expr
+  case lit p => simp [Partial.evaluate, Spec.evaluate, Spec.Expr.asPartialExpr, Except.map]
+  case var v =>
+    have h := Var.on_concrete_eqv_concrete_eval v request entities wf
+    unfold PartialEvalEquivConcreteEval at h ; exact h
+  case and x₁ x₂ =>
+    have ih₁ := on_concrete_eqv_concrete_eval x₁ request entities wf
+    have ih₂ := on_concrete_eqv_concrete_eval x₂ request entities wf
+    exact And.on_concrete_eqv_concrete_eval ih₁ ih₂
+  case or x₁ x₂ =>
+    have ih₁ := on_concrete_eqv_concrete_eval x₁ request entities wf
+    have ih₂ := on_concrete_eqv_concrete_eval x₂ request entities wf
+    exact Or.on_concrete_eqv_concrete_eval ih₁ ih₂
+  case ite x₁ x₂ x₃ =>
+    have ih₁ := on_concrete_eqv_concrete_eval x₁ request entities wf
+    have ih₂ := on_concrete_eqv_concrete_eval x₂ request entities wf
+    have ih₃ := on_concrete_eqv_concrete_eval x₃ request entities wf
+    exact Ite.on_concrete_eqv_concrete_eval ih₁ ih₂ ih₃
+  case unaryApp op x₁ =>
+    have ih₁ := on_concrete_eqv_concrete_eval x₁ request entities wf
+    exact Unary.on_concrete_eqv_concrete_eval ih₁
+  case binaryApp op x₁ x₂ =>
+    have ih₁ := on_concrete_eqv_concrete_eval x₁ request entities wf
+    have ih₂ := on_concrete_eqv_concrete_eval x₂ request entities wf
+    exact Binary.on_concrete_eqv_concrete_eval ih₁ ih₂
+  case getAttr x₁ attr =>
+    have ih₁ := on_concrete_eqv_concrete_eval x₁ request entities wf
+    exact GetAttr.on_concrete_eqv_concrete_eval ih₁
+  case hasAttr x₁ attr =>
+    have ih₁ := on_concrete_eqv_concrete_eval x₁ request entities wf
+    exact HasAttr.on_concrete_eqv_concrete_eval ih₁
+  case set xs =>
+    have ih : ∀ x ∈ xs, PartialEvalEquivConcreteEval x request entities := by
+      intro x h₁
+      have := List.sizeOf_lt_of_mem h₁
+      apply on_concrete_eqv_concrete_eval x request entities wf
+    exact Set.on_concrete_eqv_concrete_eval ih
+  case record attrs =>
+    have ih : ∀ kv ∈ attrs, PartialEvalEquivConcreteEval kv.snd request entities := by
+      intro kv h₁
+      have := List.sizeOf_lt_of_mem h₁
+      apply on_concrete_eqv_concrete_eval kv.snd request entities wf
+    exact Record.on_concrete_eqv_concrete_eval ih
+  case call xfn args =>
+    have ih : ∀ arg ∈ args, PartialEvalEquivConcreteEval arg request entities := by
+      intro arg h₁
+      have := List.sizeOf_lt_of_mem h₁
+      apply on_concrete_eqv_concrete_eval arg request entities wf
+    exact Call.on_concrete_eqv_concrete_eval ih
+termination_by expr
+decreasing_by
+  all_goals simp_wf
+  all_goals try omega
+  case _ => -- record
+    have h₂ : sizeOf kv.snd < sizeOf kv := by simp only [sizeOf, Prod._sizeOf_1] ; omega
+    apply Nat.lt_trans h₂
+    omega
+
+/--
+  `Prop` that a given `Result Partial.Value` is either a concrete value or an
+  error, not a residual
+-/
+def isValueOrError : Result Partial.Value → Prop
+  | .ok (.value _) => true
+  | .ok (.residual _) => false
+  | .error _ => true
+
+/--
+  Corollary to the above: partial evaluation with concrete inputs gives a
+  concrete value (or an error)
+-/
+theorem on_concrete_gives_concrete (expr : Spec.Expr) (request : Spec.Request) (entities : Spec.Entities)
+  (wf : request.WellFormed) :
+  isValueOrError (Partial.evaluate expr request entities)
+:= by
+  rw [on_concrete_eqv_concrete_eval expr request entities wf]
+  simp only [Except.map, isValueOrError]
+  split
+  <;> rename_i h
+  <;> split at h
+  <;> simp only [Except.ok.injEq, Except.error.injEq, Partial.Value.value.injEq] at h
+  <;> trivial
