cedar-lean/Cedar/Thm/Partial/Evaluation/Binary.lean
@@ -1,0 +1,108 @@
+/-
+ Copyright Cedar Contributors
+
+ Licensed under the Apache License, Version 2.0 (the "License");
+ you may not use this file except in compliance with the License.
+ You may obtain a copy of the License at
+
+      https://www.apache.org/licenses/LICENSE-2.0
+
+ Unless required by applicable law or agreed to in writing, software
+ distributed under the License is distributed on an "AS IS" BASIS,
+ WITHOUT WARRANTIES OR CONDITIONS OF ANY KIND, either express or implied.
+ See the License for the specific language governing permissions and
+ limitations under the License.
+-/
+
+import Cedar.Partial.Evaluator
+import Cedar.Spec.Evaluator
+import Cedar.Thm.Data.Control
+import Cedar.Thm.Data.Map
+import Cedar.Thm.Data.Set
+import Cedar.Thm.Partial.Evaluation.Basic
+
+namespace Cedar.Thm.Partial.Evaluation.Binary
+
+open Cedar.Data
+open Cedar.Spec (BinaryOp EntityUID intOrErr Result)
+
+/--
+  `Partial.Entities.ancestorsOrEmpty` on concrete entities is the same as
+  `Spec.Entities.ancestorsOrEmpty` on those entities
+-/
+theorem ancestorsOrEmpty_on_concrete_eqv_concrete {entities : Spec.Entities} {uid : EntityUID} :
+  Partial.Entities.ancestorsOrEmpty entities uid = Spec.Entities.ancestorsOrEmpty entities uid
+:= by
+  unfold Partial.Entities.ancestorsOrEmpty Spec.Entities.ancestorsOrEmpty
+  unfold Spec.Entities.asPartialEntities Spec.EntityData.asPartialEntityData
+  rw [← Map.find?_mapOnValues]
+  cases entities.find? uid <;> simp
+
+/--
+  `Partial.inₑ` on concrete arguments is the same as `Spec.inₑ` on those arguments
+-/
+theorem partialInₑ_on_concrete_eqv_concrete {uid₁ uid₂ : EntityUID} {entities : Spec.Entities} :
+  Partial.inₑ uid₁ uid₂ entities = Spec.inₑ uid₁ uid₂ entities
+:= by
+  unfold Partial.inₑ Spec.inₑ
+  cases uid₁ == uid₂ <;> simp only [Bool.true_or, Bool.false_or]
+  case false => simp [ancestorsOrEmpty_on_concrete_eqv_concrete]
+
+/--
+  `Partial.inₛ` on concrete arguments is the same as `Spec.inₛ` on those arguments
+-/
+theorem partialInₛ_on_concrete_eqv_concrete {uid : EntityUID} {vs : Set Spec.Value} {entities : Spec.Entities} :
+  Partial.inₛ uid vs entities = Spec.inₛ uid vs entities
+:= by
+  unfold Partial.inₛ Spec.inₛ
+  simp [partialInₑ_on_concrete_eqv_concrete]
+
+/--
+  `Partial.apply₂` on concrete arguments is the same as `Spec.apply₂` on those
+  arguments
+-/
+theorem partialApply₂_on_concrete_eqv_concrete {op : BinaryOp} {v₁ v₂ : Spec.Value} {entities : Spec.Entities} :
+  Partial.apply₂ op v₁ v₂ entities = (Spec.apply₂ op v₁ v₂ entities).map Partial.Value.value
+:= by
+  unfold Partial.apply₂ Spec.apply₂ Except.map
+  cases op <;> split <;> rename_i h
+  <;> simp only [false_implies, forall_const] at h
+  <;> try simp only [Except.ok.injEq, Partial.Value.value.injEq, Spec.Value.prim.injEq, Spec.Prim.bool.injEq]
+  case add | sub | mul => split <;> rename_i h <;> simp [h]
+  case mem.h_10 uid₁ uid₂ => simp [partialInₑ_on_concrete_eqv_concrete]
+  case mem.h_11 uid vs =>
+    simp only [partialInₛ_on_concrete_eqv_concrete]
+    cases Spec.inₛ uid vs entities <;> simp
+  case mem.h_12 =>
+    split <;> rename_i h₂ <;> split at h₂ <;> simp at *
+    assumption
+
+/--
+  `Partial.evaluateBinaryApp` on concrete arguments is the same as `Spec.apply₂` on
+  those arguments
+-/
+theorem evaluateBinaryApp_on_concrete_eqv_concrete {op : BinaryOp} {v₁ v₂ : Spec.Value} {entities : Spec.Entities} :
+  Partial.evaluateBinaryApp op v₁ v₂ entities = (Spec.apply₂ op v₁ v₂ entities).map Partial.Value.value
+:= by
+  simp [Partial.evaluateBinaryApp, partialApply₂_on_concrete_eqv_concrete]
+
+/--
+  Inductive argument that partial evaluating a concrete `Partial.Expr.binaryApp`
+  expression gives the same output as concrete-evaluating the
+  `Spec.Expr.binaryApp` with the same subexpressions
+-/
+theorem on_concrete_eqv_concrete_eval {x₁ x₂ : Spec.Expr} {request : Spec.Request} {entities : Spec.Entities} {op : BinaryOp} :
+  PartialEvalEquivConcreteEval x₁ request entities →
+  PartialEvalEquivConcreteEval x₂ request entities →
+  PartialEvalEquivConcreteEval (Spec.Expr.binaryApp op x₁ x₂) request entities
+:= by
+  unfold PartialEvalEquivConcreteEval
+  intro ih₁ ih₂
+  unfold Partial.evaluate Spec.evaluate Spec.Expr.asPartialExpr
+  simp only [ih₁, ih₂, Except.map]
+  cases h₁ : Spec.evaluate x₁ request entities <;> simp only [h₁, Except.bind_err, Except.bind_ok]
+  case ok v₁ =>
+    cases h₂ : Spec.evaluate x₂ request entities <;> simp only [h₂, Except.bind_err, Except.bind_ok]
+    case ok v₂ => simp [evaluateBinaryApp_on_concrete_eqv_concrete, Except.map]
+
+end Cedar.Thm.Partial.Evaluation.Binary
