cedar-lean/Cedar/Thm/Partial/Evaluation/Record.lean
@@ -1,0 +1,151 @@
+/-
+ Copyright Cedar Contributors
+
+ Licensed under the Apache License, Version 2.0 (the "License");
+ you may not use this file except in compliance with the License.
+ You may obtain a copy of the License at
+
+      https://www.apache.org/licenses/LICENSE-2.0
+
+ Unless required by applicable law or agreed to in writing, software
+ distributed under the License is distributed on an "AS IS" BASIS,
+ WITHOUT WARRANTIES OR CONDITIONS OF ANY KIND, either express or implied.
+ See the License for the specific language governing permissions and
+ limitations under the License.
+-/
+
+import Cedar.Partial.Evaluator
+import Cedar.Spec.Evaluator
+import Cedar.Thm.Data.Control
+import Cedar.Thm.Data.Map
+import Cedar.Thm.Partial.Evaluation.Basic
+
+namespace Cedar.Thm.Partial.Evaluation.Record
+
+open Cedar.Data
+open Cedar.Spec (Attr Error Result)
+
+/--
+  `Partial.bindAttr` on concrete arguments is the same as `Spec.bindAttr` on
+  those arguments
+-/
+theorem bindAttr_on_concrete_eqv_concrete {a : Attr} {res : Result Spec.Value} :
+  Partial.bindAttr a (res.map Partial.Value.value) = (Spec.bindAttr a res).map λ (k, v) => (k, Partial.Value.value v)
+:= by
+  unfold Partial.bindAttr Spec.bindAttr
+  cases res <;> simp [Except.map]
+
+/--
+  `List.mapM_pmap_subtype` specialized for a particular setting involving pairs
+  and `Spec.bindAttr`
+-/
+private theorem mapM_pmap_subtype_spec_bindAttr
+  {p : (Attr × β) → Prop}
+  (f : β → Result Spec.Value)
+  (pairs: List (Attr × β))
+  (h : ∀ pair ∈ pairs, p pair) :
+  List.mapM (λ x : {pair : (Attr × β) // p pair} => Spec.bindAttr x.val.fst (f x.val.snd)) (List.pmap Subtype.mk pairs h) =
+  pairs.mapM (λ x => Spec.bindAttr x.fst (f x.snd))
+:= by
+  rw [←List.mapM'_eq_mapM]
+  induction pairs <;> simp [*]
+
+/--
+  `List.mapM_pmap_subtype` specialized for a particular setting involving pairs
+  and `Partial.bindAttr`
+-/
+private theorem mapM_pmap_subtype_partial_bindAttr
+  {p : (Attr × β) → Prop}
+  (f : β → Result Partial.Value)
+  (pairs: List (Attr × β))
+  (h : ∀ pair ∈ pairs, p pair) :
+  List.mapM (λ x : {pair : (Attr × β) // p pair} => Partial.bindAttr x.val.fst (f x.val.snd)) (List.pmap Subtype.mk pairs h) =
+  pairs.mapM (λ x => Partial.bindAttr x.fst (f x.snd))
+:= by
+  rw [←List.mapM'_eq_mapM]
+  induction pairs <;> simp [*]
+
+/--
+  `List.mapM₂_eq_mapM` specialized for a particular setting involving pairs and
+  `Spec.bindAttr`
+-/
+private theorem mapM₂_eq_mapM_spec_bindAttr [SizeOf β]
+  (f : β → Result Spec.Value)
+  (attrs : List (Attr × β)) :
+  attrs.mapM₂
+    (λ x : {x : Attr × β // sizeOf x.snd < 1 + sizeOf attrs} => match x with
+      | ⟨(a, b), _⟩ => Spec.bindAttr a (f b)
+    ) =
+  attrs.mapM λ (a, b) => Spec.bindAttr a (f b)
+:= by
+  simp [List.mapM₂, List.attach₂, mapM_pmap_subtype_spec_bindAttr]
+
+/--
+  `List.mapM₂_eq_mapM` specialized for a particular setting involving pairs and
+  `Partial.bindAttr`
+-/
+private theorem mapM₂_eq_mapM_partial_bindAttr [SizeOf β]
+  (f : β → Result Partial.Value)
+  (attrs : List (Attr × β)) :
+  attrs.mapM₂
+    (λ x : {x : Attr × β // sizeOf x.snd < 1 + sizeOf attrs} => match x with
+      | ⟨(a, b), _⟩ => Partial.bindAttr a (f b)
+    ) =
+  attrs.mapM λ (a, b) => Partial.bindAttr a (f b)
+:= by
+  simp [List.mapM₂, List.attach₂, mapM_pmap_subtype_partial_bindAttr]
+
+/--
+  Inductive argument that partial evaluating a concrete `Partial.Expr.record`
+  expression gives the same output as concrete-evaluating the `Spec.Expr.record`
+  with the same subexpressions
+-/
+theorem on_concrete_eqv_concrete_eval {attrs : List (Attr × Spec.Expr)} {request : Spec.Request} {entities : Spec.Entities} :
+  (∀ kv ∈ attrs, PartialEvalEquivConcreteEval kv.snd request entities) →
+  PartialEvalEquivConcreteEval (Spec.Expr.record attrs) request entities
+:= by
+  unfold PartialEvalEquivConcreteEval
+  intro ih₁
+  unfold Partial.evaluate Spec.evaluate Spec.Expr.asPartialExpr
+  simp only
+  rw [List.map_attach₂_snd Spec.Expr.asPartialExpr]
+  rw [mapM₂_eq_mapM_spec_bindAttr (Spec.evaluate · request entities)]
+  rw [mapM₂_eq_mapM_partial_bindAttr (Partial.evaluate · request entities)]
+  simp only [List.mapM_map]
+  induction attrs
+  case nil => simp [Except.map, pure, Except.pure]
+  case cons kv tl ih =>
+    specialize ih (by
+      intro kv' h₁
+      exact ih₁ kv' (List.mem_cons_of_mem kv h₁)
+    )
+    cases h₁ : Spec.bindAttr kv.fst (Spec.evaluate kv.snd request entities)
+    <;> cases h₂ : Partial.bindAttr kv.fst (Partial.evaluate kv.snd request entities)
+    <;> cases h₃ : Spec.evaluate kv.snd request entities
+    <;> simp only [h₁, h₂, List.mapM_cons, Except.bind_err, Except.bind_ok, bind_assoc, pure_bind, Option.pure_def, Option.bind_eq_bind, List.map_cons, List.mapM_cons]
+    <;> simp only [ih₁ kv, Except.map, true_or, List.mem_cons] at h₂
+    <;> simp only [h₃, Spec.bindAttr, Partial.bindAttr, Except.bind_ok, Except.bind_err, Except.error.injEq, Except.ok.injEq] at h₁ h₂
+    case error.error.error e₁ e₂ e₃ =>
+      simp only [Except.map, Except.error.injEq]
+      subst h₁ h₂
+      rfl
+    case ok.ok.ok val' pval val =>
+      subst h₁ h₂
+      simp only [Option.some_bind]
+      -- the remaning goal is just a statement about `tl`, not `kv` itself
+      -- so we can dispatch it using `ih`
+      generalize h₃ : (tl.mapM λ x => Partial.bindAttr x.fst (Partial.evaluate x.snd.asPartialExpr request entities)) = pres at *
+      generalize h₄ : (tl.mapM λ x => Spec.bindAttr x.fst (Spec.evaluate x.snd request entities)) = sres at *
+      cases pres <;> cases sres
+      <;> simp only [Except.map, List.mem_cons, forall_eq_or_imp, Except.bind_ok, Except.bind_err, Except.error.injEq] at *
+      case error.error e₁ e₂ => exact ih
+      case ok.error pvals e => split at ih <;> simp at ih
+      case ok.ok pvals vals =>
+        split at ih <;> simp only [Except.ok.injEq, Partial.Value.value.injEq,
+          Spec.Value.record.injEq] at ih
+        case h_1 vals' h₂ =>
+          simp only [h₂, Option.some_bind, Except.ok.injEq, Partial.Value.value.injEq,
+            Spec.Value.record.injEq]
+          exact Map.make_cons ih
+
+end Cedar.Thm.Partial.Evaluation.Record
