cedar-lean/Cedar/Thm/Partial/Evaluation/Var.lean
@@ -1,0 +1,87 @@
+/-
+ Copyright Cedar Contributors
+
+ Licensed under the Apache License, Version 2.0 (the "License");
+ you may not use this file except in compliance with the License.
+ You may obtain a copy of the License at
+
+      https://www.apache.org/licenses/LICENSE-2.0
+
+ Unless required by applicable law or agreed to in writing, software
+ distributed under the License is distributed on an "AS IS" BASIS,
+ WITHOUT WARRANTIES OR CONDITIONS OF ANY KIND, either express or implied.
+ See the License for the specific language governing permissions and
+ limitations under the License.
+-/
+
+import Cedar.Partial.Evaluator
+import Cedar.Spec.Evaluator
+import Cedar.Thm.Data.Control
+import Cedar.Thm.Data.Map
+import Cedar.Thm.Partial.Evaluation.Basic
+
+namespace Cedar.Thm.Partial.Evaluation.Var
+
+open Cedar.Data
+open Cedar.Spec (Var)
+
+/--
+  `Partial.evaluateVar` on concrete arguments gives the same output as
+  `Spec.evaluate` on those arguments
+-/
+theorem partialEvaluateVar_on_concrete_eqv_concrete_eval (v : Var) (request : Spec.Request) (entities : Spec.Entities)
+  (wf : request.WellFormed) :
+  Partial.evaluateVar v request = (Spec.evaluate (Spec.Expr.var v) request entities).map Partial.Value.value
+:= by
+  unfold Partial.evaluateVar Spec.evaluate
+  unfold Spec.Request.WellFormed at wf
+  cases v <;> simp only [Spec.Request.asPartialRequest, Except.map]
+  case context =>
+    split
+    case h_1 m h₁ =>
+      simp only [Except.ok.injEq, Partial.Value.value.injEq, Spec.Value.record.injEq]
+      rw [← Map.eq_iff_kvs_equiv (wf₁ := by simp [Map.mapMOnValues_wf (Map.mapOnValues_wf.mp wf) h₁]) (wf₂ := wf)]
+      simp only [List.Equiv, List.subset_def]
+      constructor
+      case left =>
+        intro (k, v) h₂
+        rw [Map.mapOnValues_eq_make_map _ wf] at h₁
+        unfold Map.toList at h₁
+        replace ⟨pv, h₁, h₃⟩ := Map.mapMOnValues_some_implies_all_from_some h₁ (k, v) h₂
+        replace h₁ := Map.make_mem_list_mem h₁
+        cases pv <;> simp only [Option.some.injEq] at h₃
+        case value v =>
+          subst v
+          rw [List.mem_map] at h₁
+          replace ⟨(k', v'), h₁, h₃⟩ := h₁
+          simp only [Prod.mk.injEq, Partial.Value.value.injEq] at h₃
+          replace ⟨h₃, h₃'⟩ := h₃
+          subst k' v'
+          exact h₁
+      case right =>
+        intro (k, v) h₂
+        have ⟨v', h₃, h₄⟩ := Map.mapMOnValues_some_implies_all_some h₁ (k, v) (Map.in_kvs_in_mapOnValues h₂)
+        simp only [Option.some.injEq] at h₄
+        subst h₄
+        simp [h₃]
+    case h_2 h₁ =>
+      exfalso
+      replace ⟨v, h₁, h₂⟩ := Map.mapMOnValues_none_iff_exists_none.mp h₁
+      cases v <;> simp only at h₂
+      case residual r =>
+        rw [Map.mapOnValues_eq_make_map _ wf] at h₁
+        replace h₁ := Map.mem_values_make h₁
+        simp [List.mem_map] at h₁
+
+/--
+  Partial-evaluating a concrete `Var` expression gives the same output as
+  concrete-evaluating the `Var`
+-/
+theorem on_concrete_eqv_concrete_eval (v : Var) (request : Spec.Request) (entities : Spec.Entities)
+  (wf : request.WellFormed) :
+  PartialEvalEquivConcreteEval (Spec.Expr.var v) request entities
+:= by
+  unfold PartialEvalEquivConcreteEval Spec.Expr.asPartialExpr Partial.evaluate
+  exact partialEvaluateVar_on_concrete_eqv_concrete_eval v request entities wf
+
+end Cedar.Thm.Partial.Evaluation.Var
